mechanization/theories/Core/Soundness/TermStructureCases.v
@@ -5,103 +5,134 @@ From McPTS.Core.Semantic Require Import Realizability.
 From McPTS.Core.Soundness Require Import LogicalRelation.
 Import Domain_Notations.
 
-Lemma presup_glu_rel_exp : forall {Γ M A},
-    {{ Γ ⊩ M : A }} ->
-    {{ ⊩ Γ }} /\ (exists i, {{ Γ ⊩ A : Type@i }}).
+Lemma presup_glu_rel_exp {P} (pred_P : PredicativeSig P) (full_P : FullSig P) : forall {sts Γ M A},
+    {{ ⟪ pred_P ⟫ Γ : sts ⊩ M : A }} ->
+    {{ ⟪ pred_P ⟫ ⊩ Γ : sts }} /\ (exists s, {{ ⟪ pred_P ⟫ Γ : sts ⊩ A : Sort@s }}).
 Proof.
   intros * [? [? []]].
   split; [eexists; eassumption |].
   do 2 eexists; intuition.
+  assert (exists s', Ax P x0 s') by (eapply full_P; mauto).
+  destruct_conjs.  
   eexists; mauto 4.
 Qed.
 
-Lemma presup_ctx_glu_rel_exp : forall {Γ M A},
-    {{ Γ ⊩ M : A }} ->
-    {{ ⊩ Γ }}.
+Lemma presup_ctx_glu_rel_exp {P} (pred_P : PredicativeSig P) (full_P : FullSig P) : forall {sts Γ M A},
+    {{ ⟪ pred_P ⟫ Γ : sts ⊩ M : A }} ->
+    {{ ⟪ pred_P ⟫ ⊩ Γ : sts }}.
 Proof.
-  intros * []%presup_glu_rel_exp.
-  eassumption.
+  intros * []%presup_glu_rel_exp;
+    eassumption.
 Qed.
 
 #[export]
 Hint Resolve presup_ctx_glu_rel_exp : mcpts.
 
-Lemma presup_typ_glu_rel_exp : forall {Γ M A},
-    {{ Γ ⊩ M : A }} ->
-    exists i, {{ Γ ⊩ A : Type@i }}.
+Lemma presup_typ_glu_rel_exp {P} (pred_P : PredicativeSig P) (full_P : FullSig P) : forall {sts Γ M A},
+    {{ ⟪ pred_P ⟫ Γ : sts ⊩ M : A }} ->
+    exists s, {{ ⟪ pred_P ⟫ Γ : sts ⊩ A : Sort@s }}.
 Proof.
-  intros * []%presup_glu_rel_exp.
-  eassumption.
+  intros * []%presup_glu_rel_exp;
+    eassumption.
 Qed.
 
 #[export]
 Hint Resolve presup_typ_glu_rel_exp : mcpts.
 
-Lemma glu_rel_exp_vlookup : forall {Γ x A},
-    {{ ⊩ Γ }} ->
+Lemma glu_rel_exp_vlookup {P} (pred_P : PredicativeSig P) (full_P : FullSig P) : forall {sts Γ x A},
     {{ #x : A ∈ Γ }} ->
-    {{ Γ ⊩ #x : A }}.
+    {{ ⟪ pred_P ⟫ ⊩ Γ : sts }} ->
+    {{ ⟪ pred_P ⟫ Γ : sts ⊩ #x : A }}.
 Proof.
-  intros * [Sb] Hx. gen Sb.
-  induction Hx; intros;
-    match_by_head1 glu_ctx_env ltac:(fun H => invert_glu_ctx_env H).
+  intros * Hx.
+  gen sts.
+  induction Hx; intros * [Sb];
+    match_by_head1 (@glu_ctx_env P) ltac:(fun H => invert_glu_ctx_env H).
+
+  
+  (* intros * [Sb] Hx. gen Sb. *)
+  (* induction Hx; intros; *)
+  (*   match_by_head1 (@glu_ctx_env P) ltac:(fun H => invert_glu_ctx_env H). *)
   - eexists.
     split; [econstructor |]; try reflexivity; mauto.
     eexists.
     intros.
-    destruct_by_head cons_glu_sub_pred.
+    destruct_by_head (@cons_glu_sub_pred P).
     econstructor; mauto.
-  - assert {{ Γ ⊩ #n : A }} as Hn by mauto.
-    assert (exists i, {{ Γ ⊢ A : Type@i }}) as [j] by (gen_presups; mauto 3).
+  - assert (glu_ctx_env pred_P {{{ sts, s }}} Sb {{{ Γ, B }}}) by (econstructor; mauto).
+    assert {{ ⟪ pred_P ⟫ Γ : sts ⊩ #n : A }} as Hn.
+    {
+      eapply IHHx.
+      econstructor; eauto.
+    }
+    
+    assert (exists s, {{ Γ ⊢ A : Sort@s }}) as [s'] by (gen_presups; mauto 3).
     invert_glu_rel_exp Hn.
     rename x into k.
     eexists.
-    split; [econstructor |]; try reflexivity; mauto.
-    eexists (max j k).
-    intros.
-    destruct_by_head cons_glu_sub_pred.
-    destruct_glu_rel_exp_with_sub.
-    simplify_evals.
-    rename a into b.
-    rename a0 into a.
-    assert {{ Dom a ≈ a ∈ per_univ k }} as [] by mauto.
-    eapply mk_glu_rel_exp_with_sub''; intuition mauto using per_univ_elem_cumu_max_right.
-    assert {{ ⊢ Γ, B }} by mauto 3.
-    assert {{ Δ ⊢ A[Wk][σ] ≈ A[Wk∘σ] : Type@j }} by mauto 3.
-    assert {{ Δ ⊢ A[Wk][σ] ≈ A[Wk∘σ] : Type@(max j k) }} as -> by mauto 3 using lift_exp_eq_max_left.
-    assert {{ Γ ⊢ #n : A }} by mauto 4.
-    assert {{ Γ, B ⊢ #n[Wk] : A[Wk] }} by mauto 3.
-    assert {{ Γ, B ⊢ #n[Wk] ≈ #(S n) : A[Wk] }} by mauto 3.
-    assert {{ Δ ⊢ #n[Wk][σ] ≈ #(S n)[σ] : A[Wk∘σ] }} as <- by (eapply wf_exp_eq_conv; mauto 3).
-    assert {{ Δ ⊢ #n[Wk∘σ] ≈ #n[Wk][σ] : A[Wk∘σ] }} as <- by mauto 3.
-    eapply glu_univ_elem_exp_cumu_max_right; revgoals; mautosolve 4.
+    split.
+    + econstructor; try reflexivity; mauto.
+      intros.
+      dependent destruction H3.
+      handle_functional_glu_ctx_env P.
+      eapply H5.
+      eassumption.
+    + eexists.
+      intros.
+      destruct_by_head (@cons_glu_sub_pred P).
+      destruct_glu_rel_exp_with_sub.
+      simplify_evals.
+      rename a into b.
+      rename a0 into a.
+      assert {{ Dom a ≈ a ∈ per_sort pred_P x0 }} as [] by mauto.
+      eapply mk_glu_rel_exp_with_sub''; intuition mauto.
+      handle_functional_glu_sort_elem P.
+      
+      
+      assert {{ ⊢ Γ, B }} by mauto 3.
+      assert {{ Δ ⊢ A[Wk][σ] ≈ A[Wk∘σ] : Sort@s' }} by mauto.
+      assert {{ Γ ⊢ A : Sort@x0 }} by mauto.
+      assert {{ Δ ⊢ A[Wk][σ] ≈ A[Wk∘σ] : Sort@x0 }} as -> by mauto.
+      assert {{ Γ ⊢ #n : A }} by mauto 4.
+      assert {{ Γ, B ⊢ #n[Wk] : A[Wk] }} by mauto 3.
+      assert {{ Γ, B ⊢ #n[Wk] ≈ #(S n) : A[Wk] }} by mauto 3.
+      assert {{ Δ ⊢ #n[Wk][σ] ≈ #(S n)[σ] : A[Wk∘σ] }} as <- by (eapply wf_exp_eq_conv; mauto).
+      assert {{ Δ ⊢ #n[Wk∘σ] ≈ #n[Wk][σ] : A[Wk∘σ] }} as <- by mauto 3.
+      eassumption.
 Qed.
 
 #[export]
 Hint Resolve glu_rel_exp_vlookup : mcpts.
 
-Lemma glu_rel_exp_sub : forall {Γ σ Δ M A},
-    {{ Γ ⊩s σ : Δ }} ->
-    {{ Δ ⊩ M : A }} ->
-    {{ Γ ⊩ M[σ] : A[σ] }}.
+Lemma glu_rel_exp_sub {P} (pred_P : PredicativeSig P) (full_P : FullSig P) : forall {sts Γ σ Δ sts' M A},
+    {{ ⟪ pred_P ⟫ Γ : sts ⊩s σ : Δ : sts' }} ->
+    {{ ⟪ pred_P ⟫ Δ : sts' ⊩ M : A }} ->
+    {{ ⟪ pred_P ⟫ Γ : sts ⊩ M[σ] : A[σ] }}.
 Proof.
   intros * Hσ HM.
   assert {{ Γ ⊢s σ : Δ }} by mauto 3.
   assert {{ Δ ⊢ M : A }} by mauto 3.
-  assert (exists i, {{ Δ ⊩ A : Type@i }}) as [i] by mauto 3.
+  assert (exists s, {{ ⟪ pred_P ⟫ Δ : sts' ⊩ A : Sort@s }}) as [s] by mauto 3.
   destruct Hσ as [SbΓ [SbΔ]].
   destruct_conjs.
   invert_glu_rel_exp HM.
-  assert {{ Δ ⊢ A : Type@i }} by mauto 3.
+  assert {{ Δ ⊢ A : Sort@s }} by mauto 3.
   eexists; split; mauto.
   eexists.
   intros Δ' τ ρ ?.
   destruct_glu_rel_sub_with_sub.
+  handle_functional_glu_ctx_env P.
+  rewrite <- H12 in H10.
   destruct_glu_rel_exp_with_sub.
-  assert {{ Dom a ≈ a ∈ per_univ i }} as [] by mauto.
+  assert {{ Dom a ≈ a ∈ per_sort pred_P x0 }} as [] by mauto.
   econstructor; mauto.
   assert {{ Δ' ⊢s τ : Γ }} by mauto 3.
-  assert {{ Δ' ⊢ A[σ][τ] ≈ A[σ∘τ] : Type@i }} as -> by mauto 3.
+  assert {{ Δ' ⊢ A[σ∘τ] : Sort@x0 }} by (eapply glu_sort_elem_trm_sort_lvl; mauto).
+  assert (exists Δ'' K, {{ Δ' ⊢s σ∘τ : Δ'' }} /\ {{ Δ'' ⊢ A : K }} /\ {{ Δ' ⊢ K[σ∘τ] ≈ Sort@x0 }}) by mauto.
+  destruct H18 as [Δ'' [? []]].
+  assert (exists Δ''', {{ Δ' ⊢s τ : Δ''' }} /\ {{ Δ''' ⊢s σ : Δ'' }}) by mauto.
+  destruct_conjs.
+  assert {{ Δ' ⊢ A[σ][τ] ≈ A[σ∘τ] : Sort@x0 }} as -> by (symmetry; mauto).
   assert {{ Δ' ⊢ M[σ][τ] ≈ M[σ∘τ] : A[σ∘τ] }} as ->; mauto 3.
 Qed.
 
